\bigskip
\section*{RÃ©ponses}

\begin{reponse}{4.1}
    \begin{inparaenum}
    \item $\bar{X}$
    \item $\bar{X}/(1 - \bar{X})$
    \item $\bar{X}$
    \item $\bar{X}$
    \item $\bar{X} - 1$
    \end{inparaenum}
  
\end{reponse}
\begin{reponse}{4.2}
b) $\hat \mu = \ln\left\{\frac{\bar Y_n^2}{\sqrt{\frac{1}{n}\sum_{i=1}^n Y_i^2}} \right\}$ et $\hat\sigma^2 = \ln\left\{\frac{\frac{1}{n}\sum_{i=1}^n Y_i^2}{\bar Y_n^2} \right\}$
\end{reponse}
\begin{reponse}{4.3}
    $0,2381$.
  
\end{reponse}
\begin{reponse}{4.4}
    \begin{inparaenum}
    \item $\hat{\theta} = 2 \bar{X} - 1$
    \item $9,5$
    \end{inparaenum}
  
\end{reponse}
\begin{reponse}{4.5}
$\hat{\mu}=3,241$, $\hat{\sigma}=0,4$ et $\widehat{\Pr(X>30)}= 0,3446$
\end{reponse}
\begin{reponse}{4.6}
$\hat{\tau}=2$ et $\hat{\theta}=200$
\end{reponse}
\begin{reponse}{4.7}
13,75
\end{reponse}
\begin{reponse}{4.8}
    \begin{inparaenum}
    \item $\bar{X}$
    \item $-n/\ln(X_1 \cdots X_n)$
    \item $\bar{X}$
    \item $\text{med}(X_1, \dots, X_n)$
    \item $X_{(1)}$
    \end{inparaenum}
  
\end{reponse}
\begin{reponse}{4.9}
    \begin{enumerate}
    \item $\esp{X} = \mu + \lambda^{-1}$, $\var{X} = \lambda^{-2}$
    \item $\hat{\mu} = X_{(1)}$, $\hat{\lambda} = n/\sum_{i = 1}^n (X_i -
        X_{(1)})$
    \end{enumerate}
  
\end{reponse}
\begin{reponse}{4.11}
    $\hat{\mu} = \bar{X}$, $\hat{\lambda} = n/\sum_{i = 1}^n
    (X_i^{-1} - \bar{X}^{-1})$
  
\end{reponse}
\begin{reponse}{4.12}
a) $\ex[X_1]= \theta/(\alpha-1)$ et $
\vr(X_1)=\alpha\theta^2/\{(\alpha-1)^2(\alpha-2)\}$

b) $\hat\alpha = 2S_n^2/(S_n^2-\bar X_n^2)$ et $\hat\theta=\bar X_n (S_n^2+\bar X_n^2)/(S_n^2-\bar X_n^2)$
\end{reponse}
\begin{reponse}{4.13}
    $\hat{a} = \min(X_1, \dots, X_n)$ et $\hat{b} = \max(X_1, \dots,
    X_n)$
  
\end{reponse}
\begin{reponse}{4.14}
a) $\{\max(X_1,\dots,X_n) -1\}/2$
b) $\{\max(X_1,\dots,X_n)\}^2/12$
\end{reponse}
\begin{reponse}{4.15}
    \begin{enumerate}
    \item $\tilde{\theta} = \bar{X}$, $\hat{\theta} =
      \min(\bar{X}, 1/2)$
    \item EQM$(\tilde{\theta}) = \theta (1 - \theta)/n$,
      EQM$(\hat{\theta}) =
      \sum_{y = 0}^{[n/2]} (y/n - \theta)^2 \binom{n}{y} \theta^y (1 -
      \theta)^{n-y} + \sum_{y = [n/2] + 1}^n (1/2 - \theta)^2
      \binom{n}{y} \theta^y (1 - \theta)^{n - y}$
    \item EQM$(\hat{\theta}) \leq$ EQM$(\tilde{\theta})$
    \end{enumerate}
  
\end{reponse}
\begin{reponse}{4.16}
b) $\hat \mu =6.969$ et $\hat\sigma^2 =1.112$
c) $\hat\alpha =3.922$ et
$\hat\theta=5414.77$
d) Log-normale~: $114~374,2$, Pareto~: $115~004,2$
f) 11~296,76,  14~166,68,  12~720,54  et  16~537,1
\end{reponse}
