\bigskip
\section*{RÃ©ponses}

\begin{reponse}{1.1}
a) non \, \, b) oui
\end{reponse}
\begin{reponse}{1.3}
    \begin{inparaenum}
    \item $f(x) = \alpha \beta x^{\alpha - 1}e^{-\beta x^{\alpha}}$
    \item $\esp{X} = \beta^{-1/\alpha} \Gamma(1 + 1/\alpha)$, %
      $\var{X} = \beta^{-2/\alpha} (\Gamma(1 + 2/\alpha) -
      \Gamma(1 + 1/\alpha)^2)$
    \end{inparaenum}
  
\end{reponse}
\begin{reponse}{1.4}
$\ex(X)=\alpha/(\alpha+\beta)$ et $\Var{X}=(\alpha\beta)/\{(\alpha+\beta)^2(\alpha+\beta+1)\}$
\end{reponse}
\begin{reponse}{1.5}
$M_X(t) = \exp\{\lambda(e^t-1)\}$ pour tout $t \in \mathbb{R}$.
\end{reponse}
\begin{reponse}{1.6}
     b) 0.2775 \, \, c) 21~000
   
\end{reponse}
\begin{reponse}{1.7}
    $c = \mu$
  
\end{reponse}
\begin{reponse}{1.9}
Non.
\end{reponse}
\begin{reponse}{1.10}
1/5
\end{reponse}
\begin{reponse}{1.11}
    $F_{X_{(1)}}(x) = 1 - (1 -  F_X(x))^n$
  
\end{reponse}
\begin{reponse}{1.12}
    $1 - (1 - e^{-3})^4$
  
\end{reponse}
\begin{reponse}{1.13}
    $1/8$
  
\end{reponse}
\begin{reponse}{1.15}
    $X_{(1)} \sim \text{Weibull}(\alpha, n\beta)$.
  
\end{reponse}
\begin{reponse}{1.16}
$f_{X_{(1)}, X_{(n)}}(x,y) = n (n - 1) (F(y) - F(x))^{n - 2}  f(x) f(y), \quad x<y$
\end{reponse}
\begin{reponse}{1.17}
$f_{R, T}(r, t) = n (n - 1)\{ F_X(t + r/2) - F_X(t - r/2)\}^{n - 2}
    f_X(t + r/2) f_X(t - r/2),$

pour $r > 0$ et $-\infty < t < \infty$.
\end{reponse}
\begin{reponse}{1.19}
    $5/16$
  
\end{reponse}
\begin{reponse}{1.20}
    $7/12$
  
\end{reponse}
\begin{reponse}{1.21}
    $1/2$.
  
\end{reponse}
\begin{reponse}{1.22}
     \begin{enumerate}
     \item $\esp{R} = (n - 1)/(n + 1)$ et $\var{R} = (2n - 2)/[(n +
       1)^2 (n + 2)]$.
     \item $\esp{T} = 1/2$ et $\var{T} = 1/[2 (n + 1)(n + 2)]$.
     \end{enumerate}
   
\end{reponse}
